src/Examples/QueryStructure/ProcessScheduler.v
@@ -36,30 +36,924 @@ Definition SchedulerSpec : ADT _ :=
       ret (r, proc)
               }%methDefParsing.
 
-Definition SharpenedScheduler :
-  MostlySharpened SchedulerSpec.
+Record DelegationADT (Sig : ADTSig)
+  : Type
+  := Build_SharpenedUnderDelegates
+       { DelegateeIDs : nat;
+         DelegateeSigs : Fin.t DelegateeIDs -> ADTSig;
+         DelegatedImplementation :
+           forall (DelegateImpls : forall idx,
+                      ADT (DelegateeSigs idx)),
+             ADT Sig;
+         DelegateeSpecs : forall idx, ADT (DelegateeSigs idx) }.
+
+Definition refinedUnderDelegates
+           (Sig : ADTSig)
+           (spec : ADT Sig)
+           (adt : DelegationADT Sig)
+  := forall (DelegateImpls : forall idx,
+                ADT (DelegateeSigs adt idx))
+            (ValidImpls
+             : forall idx : Fin.t (DelegateeIDs adt),
+                refineADT (DelegateeSpecs adt idx)
+                          (DelegateImpls idx)),
+    refineADT spec
+              (DelegatedImplementation adt DelegateImpls).
+
+Definition refinedUnderDelegatesStep
+           (Sig : ADTSig)
+           (spec adt' : ADT Sig)
+           (dadt : DelegationADT Sig)
+           (refine_spec : refineADT spec adt')
+           (refine_adt' : refinedUnderDelegates adt' dadt)
+  : refinedUnderDelegates spec dadt.
+      unfold refinedUnderDelegates; intros.
+      eapply transitivityT; eauto.
+Defined.
+
+Lemma Notation_Friendly_refinedUnderDelegates
+           (RepT : Type)
+           {DelegateIDs n n'}
+           (consSigs : Vector.t consSig n)
+           (methSigs : Vector.t methSig n')
+           (consDefs : ilist consSigs)
+           (methDefs : ilist methSigs)
+           (DelegateSigs : Fin.t DelegateIDs -> ADTSig)
+           (rep : (Fin.t DelegateIDs -> Type) -> Type)
+           (refinedConstructors :
+              forall
+                (DelegateImpls : forall idx, ADT (DelegateSigs idx)),
+                ilist
+                  (B := fun Sig : consSig =>
+                          constructorType
+                            (rep (fun idx => Rep (DelegateImpls idx)))
+                            (consDom Sig)) consSigs)
+           (refinedMethods :
+              forall (DelegateImpls : forall idx, ADT (DelegateSigs idx)),
+                ilist
+                  (B := fun Sig : methSig =>
+                          methodType
+                            (rep (fun idx => Rep (DelegateImpls idx)))
+                            (methDom Sig)
+                            (methCod Sig)) methSigs)
+           (DelegateSpecs : forall idx, ADT (DelegateSigs idx))
+           (cAbsR :
+              forall
+                (DelegateImpls : forall idx, ADT (DelegateSigs idx))
+                (ValidImpls
+                 : forall idx : Fin.t DelegateIDs,
+                    refineADT (DelegateSpecs idx)
+                              (DelegateImpls idx)),
+                RepT -> rep (fun idx => Rep (DelegateImpls idx)) -> Prop)
+           (constructorsRefinesSpec :
+              forall
+                (DelegateImpls : forall idx, ADT (DelegateSigs idx))
+                (ValidImpls
+                 : forall idx : Fin.t DelegateIDs,
+                    refineADT (DelegateSpecs idx)
+                              (DelegateImpls idx)),
+                Iterate_Dep_Type_BoundedIndex
+                  (fun idx =>
+                     @refineConstructor
+                       (RepT)
+                       (rep (fun idx => Rep (DelegateImpls idx)))
+                       (cAbsR _ ValidImpls)
+                       (consDom (Vector.nth consSigs idx))
+                       (getConsDef consDefs idx)
+                       (ith (refinedConstructors DelegateImpls) idx)))
+           (methodsRefinesSpec :
+              forall
+                (DelegateImpls : forall idx, ADT (DelegateSigs idx))
+                (ValidImpls
+                 : forall idx : Fin.t DelegateIDs,
+                    refineADT (DelegateSpecs idx)
+                              (DelegateImpls idx)),
+                Iterate_Dep_Type_BoundedIndex
+                  (fun idx =>
+                     @refineMethod
+                       (RepT)
+                       (rep (fun idx => Rep (DelegateImpls idx)))
+                       (cAbsR _ ValidImpls)
+                       (methDom (Vector.nth methSigs idx))
+                       (methCod (Vector.nth methSigs idx))
+                       (getMethDef methDefs idx)
+                       (ith (refinedMethods DelegateImpls) idx)))
+  : refinedUnderDelegates
+      (BuildADT consDefs methDefs)
+      {|
+        DelegateeSigs := DelegateSigs;
+        DelegatedImplementation :=
+          fun DelegateImpls =>
+            BuildADT (Rep := rep (fun idx => Rep (DelegateImpls idx)))
+                     (imap (@Build_consDef _) (refinedConstructors DelegateImpls))
+                     (imap (@Build_methDef _) (refinedMethods DelegateImpls));
+        DelegateeSpecs := DelegateSpecs |}.
+      unfold refinedUnderDelegates; simpl; intros.
+      eapply (@refinesADT _ (BuildADT (Rep := RepT) consDefs methDefs)
+                          (BuildADT (Rep := rep (fun idx => Rep (DelegateImpls idx))) _ _)
+                          (cAbsR DelegateImpls ValidImpls)).
+      - intros.
+        unfold Constructors; simpl.
+        rewrite <- ith_imap; eauto.
+        eapply (Lookup_Iterate_Dep_Type
+                  _ (constructorsRefinesSpec DelegateImpls ValidImpls) idx).
+      - intros.
+        unfold Methods; simpl.
+        rewrite <- ith_imap; eauto.
+        eapply (Lookup_Iterate_Dep_Type
+                 _ (methodsRefinesSpec DelegateImpls ValidImpls) idx).
+Defined.
+
+(* Sharpen_w_Delegates constructs a refinement of an ADT whose *)
+(* representation is parameterized over some abstract models of state. *)
+Definition
+  Sharpen_w_Delegates
+  (* The fixed set of 'abstract' types in the ADT's *)
+  (* representation. *)
+  (DelegateIDs : nat)
+  (AbstractReps : Fin.t DelegateIDs -> Type)
+
+  (* The parameterized representation type. Intuitively, *)
+  (* this relation swaps in 'concrete' types for the *)
+  (* abstract ones, i.e. lists for sets. The type's *)
+  (* parametricity is witnessed by FunctorRepT. *)
+  (pRepT : (Fin.t DelegateIDs -> Type) -> Type)
+
+  (* The initial representation type. *)
+  (RepT := pRepT AbstractReps)
+
+  (* The constructors and methods of the ADT being *)
+  (* sharpened. *)
+  {n n'}
+  (consSigs : Vector.t consSig n)
+  (methSigs : Vector.t methSig n')
+  (consDefs : ilist (B := consDef (Rep := RepT)) consSigs)
+  (methDefs : ilist (B := methDef (Rep := RepT)) methSigs)
+
+
+  (* The signatures of each delegate's constructors *)
+  (* and methods in terms of the abstract representation *)
+  (* types. *)
+  (numDelegateConstructors : Fin.t DelegateIDs -> nat)
+  (DelegateConstructorSigs
+   : forall (idx : Fin.t DelegateIDs),
+      Vector.t consSig (numDelegateConstructors idx))
+  (numDelegateMethods : Fin.t DelegateIDs -> nat)
+  (DelegateMethodSigs
+   : forall (idx : Fin.t DelegateIDs),
+      Vector.t methSig (numDelegateMethods idx))
+  (DelegateSigs := fun idx =>
+                     BuildADTSig
+                       (DelegateConstructorSigs idx)
+                       (DelegateMethodSigs idx))
+
+  (* The specifications of each delegate's constructors *)
+  (* and methods in terms of the abstract representation *)
+  (* types. *)
+  (DelegateConstructorSpecs
+   : forall (idx : Fin.t DelegateIDs),
+      ilist (B := consDef (Rep := AbstractReps idx))
+            (DelegateConstructorSigs idx))
+  (DelegateMethodSpecs
+   : forall (idx : Fin.t DelegateIDs),
+      ilist (B := methDef (Rep := AbstractReps idx))
+            (DelegateMethodSigs idx))
+  (DelegateSpecs := fun idx =>
+                      BuildADT
+                        (DelegateConstructorSpecs idx)
+                        (DelegateMethodSpecs idx))
+
+  (* An abstraction relation between the original representation *)
+  (* and the abstract representation (generally equality). This is *)
+  (* generically lifted to a relation between the original *)
+  (* representation and the concrete representation. *)
+  (pAbsR : forall (A B : Fin.t DelegateIDs -> Type),
+      (forall idx, A idx -> B idx -> Prop)
+      -> pRepT A -> pRepT B -> Prop)
+  (cAbsR :=
+     fun DelegateImpls'
+         (ValidImpls'
+          : forall idx : Fin.t DelegateIDs,
+             refineADT (DelegateSpecs idx)
+                       (DelegateImpls' idx))
+         r_o r_n =>
+       pAbsR _ _ (fun idx => AbsR (ValidImpls' idx)) r_o r_n)
+
+  cConstructors
+  cMethods
+  cConstructorsRefinesSpec
+  cMethodsRefinesSpec
+
+  (* The implementations of each delegate. *)
+  (ConcreteReps : Fin.t DelegateIDs -> Type)
+  (DelegateImpls : forall idx,
+      ADT (DelegateSigs idx))
+  (ValidImpls
+   : forall idx : Fin.t DelegateIDs,
+      refineADT (DelegateSpecs idx)
+                (DelegateImpls idx))
+
+  := Notation_Friendly_refinedUnderDelegates
+       consSigs methSigs
+       consDefs methDefs
+       DelegateSigs pRepT
+       cConstructors
+       cMethods
+       DelegateSpecs cAbsR
+       cConstructorsRefinesSpec
+       cMethodsRefinesSpec.
+
+Fixpoint Iterate_Dep_Type_AbsR {n}
+         (A B : Fin.t n -> Type)
+         (AB_AbsR : forall idx, A idx -> B idx -> Prop)
+         (a : Iterate_Dep_Type_BoundedIndex A)
+         (b : Iterate_Dep_Type_BoundedIndex B)
+  : Prop :=
+  match n as n' return
+        forall (A B : Fin.t n' -> Type)
+               (AB_AbsR : forall idx, A idx -> B idx -> Prop),
+          Iterate_Dep_Type_BoundedIndex A
+          -> Iterate_Dep_Type_BoundedIndex B
+          -> Prop with
+  | S n' => fun A B AB_AbsR a b =>
+              AB_AbsR _ (prim_fst a) (prim_fst b)
+              /\ Iterate_Dep_Type_AbsR (fun n' => A (Fin.FS n'))
+                                       (fun n' => B (Fin.FS n'))
+                                       (fun n' => AB_AbsR (Fin.FS n'))
+                                       (prim_snd a)
+                                       (prim_snd b)
+  | _ => fun _ _ _ _ _ => True
+  end A B AB_AbsR a b.
+
+Fixpoint UnConstryQueryStructure_Abstract_AbsR'
+         {n}
+         {qsSchema}
+         (r_o : ilist2 (B := (fun ns : RawSchema => RawUnConstrRelation (rawSchemaHeading ns))) qsSchema)
+         (r_n : Iterate_Dep_Type_BoundedIndex
+                  (fun idx : Fin.t n=>
+                     @IndexedEnsemble
+                       (@RawTuple
+                          (rawSchemaHeading (Vector.nth qsSchema idx)))))
+  : Prop :=
+  match qsSchema as qsSchema return
+        forall
+          (r_o : ilist2 (B := (fun ns : RawSchema => RawUnConstrRelation (rawSchemaHeading ns))) qsSchema)
+          (r_n : Iterate_Dep_Type_BoundedIndex
+                   (fun idx : Fin.t _ =>
+                      @IndexedEnsemble
+                        (@RawTuple
+                           (rawSchemaHeading (Vector.nth qsSchema idx))))), Prop with
+  | Vector.cons sch _ qsSchema' =>
+    fun r_o r_n =>
+      ilist2_hd r_o = prim_fst r_n
+      /\ UnConstryQueryStructure_Abstract_AbsR'
+           (prim_snd r_o)
+           (prim_snd r_n)
+  | Vector.nil  => fun _ _ => True
+  end r_o r_n.
+
+Definition UnConstryQueryStructure_Abstract_AbsR
+           {qsSchema}
+           (r_o : UnConstrQueryStructure qsSchema)
+           (r_n : Iterate_Dep_Type_BoundedIndex _)
+  := UnConstryQueryStructure_Abstract_AbsR' r_o r_n.
+
+Lemma UpdateUnConstrRelation_Abstract_AbsR {qsSchema}
+  : forall (r_o : UnConstrQueryStructure qsSchema)
+           (r_n : Iterate_Dep_Type_BoundedIndex _),
+    UnConstryQueryStructure_Abstract_AbsR r_o r_n
+    -> forall idx R,
+      UnConstryQueryStructure_Abstract_AbsR
+        (UpdateUnConstrRelation r_o idx R)
+        (Update_Iterate_Dep_Type idx _ r_n R).
+Admitted.
+
+Ltac UpdateUnConstrRelation_Abstract :=
+  match goal with
+    H : UnConstryQueryStructure_Abstract_AbsR ?r_o ?r_n
+    |- context [{ r_n | UnConstryQueryStructure_Abstract_AbsR
+                          (UpdateUnConstrRelation ?r_o ?idx ?R) r_n }] =>
+    refine pick val _;
+      [ | apply (UpdateUnConstrRelation_Abstract_AbsR r_o r_n H idx R); eauto]
+  end.
+
+Ltac PickUnchangedRep :=
+  match goal with
+    |- context [Pick (fun r_n => @?R r_n)] =>
+    match goal with
+      H : ?R' ?r_n |- _ => unify R R'; refine pick val r_n; [ | apply H]
+    end
+  end.
+
+Lemma GetUnConstrRelation_Abstract_AbsR {qsSchema}
+  : forall (r_o : UnConstrQueryStructure qsSchema)
+           (r_n : Iterate_Dep_Type_BoundedIndex _),
+    UnConstryQueryStructure_Abstract_AbsR r_o r_n
+    -> forall idx,
+      GetUnConstrRelation r_o idx = Lookup_Iterate_Dep_Type _ r_n idx.
 Proof.
-  start sharpening ADT.
+Admitted.
+
+Ltac GetUnConstrRelation_Abstract :=
+  match goal with
+    H : UnConstryQueryStructure_Abstract_AbsR ?r_o ?r_n
+    |- context [GetUnConstrRelation ?r_o ?idx] =>
+    rewrite (GetUnConstrRelation_Abstract_AbsR r_o r_n H idx)
+  end.
+
+Ltac parameterize_query_structure :=
+        repeat first
+               [ simplify with monad laws; cbv beta; simpl
+               | rewrite refine_If_Then_Else_Bind
+               | GetUnConstrRelation_Abstract
+               | UpdateUnConstrRelation_Abstract
+               | progress unfold QSDeletedTuples
+               | PickUnchangedRep].
+
+Ltac makeEvar T k :=
+  let x := fresh in evar (x : T); let y := eval unfold x in x in clear x; k y.
+
+Ltac Iterate_Dep_Type_BoundedIndex_evar n T k :=
+  match n with
+  | 0 => k tt
+  | S ?n' =>
+    Iterate_Dep_Type_BoundedIndex_evar
+      n' (fun n' => T (Fin.FS n'))
+      ltac:(fun b =>
+              makeEvar
+                (T Fin.F1)
+                ltac:(fun a =>
+                        k ({| prim_fst := a;
+                              prim_snd := b |})))
+  end.
+
+Ltac make_Vector_of_evar n T k :=
+  match n with
+  | 0 => k (@Vector.nil T)
+  | S ?n' => make_Vector_of_evar
+               n' T
+               ltac:(fun l =>
+                       makeEvar
+                         T
+                         ltac:(fun a => k (@Vector.cons T a n' l)))
+  end.
+
+Ltac ilist_of_evar' n C B As k :=
+  match n with
+  | 0 => k (fun (c : C) => @inil _ (B c))
+  | S ?n' =>
+    makeEvar (forall c : C, B c (Vector.hd As))
+             ltac:(fun b =>
+                     ilist_of_evar'
+                       n' C B (Vector.tl As)
+                       ltac:(fun Bs' => k (fun c => icons (a := Vector.hd As) (b c) (Bs' c))))
+  end.
+
+Ltac FullySharpenEachMethod_w_Delegates
+     DelegateIDs'
+     AbstractReps
+     dRepT
+     dAbsR :=
+  match goal with
+    |- refinedUnderDelegates (@BuildADT ?Rep' ?n ?n' ?consSigs ?methSigs ?consDefs ?methDefs) _ =>
+(* We build a bunch of evars in order to decompose the goal *)
+    (* into a single subgoal for each constructor. *)
+    let DelegateIDs := (eval compute in DelegateIDs') in
+    make_Vector_of_evar DelegateIDs nat
+                        ltac:(fun numDelegateConstructors' =>
+        let numDelegateConstructors := constr:(Vector.nth numDelegateConstructors') in
+    make_Vector_of_evar DelegateIDs nat
+      ltac:(fun numDelegateMethods' =>
+        let numDelegateMethods := constr:(Vector.nth numDelegateMethods') in
+    Iterate_Dep_Type_BoundedIndex_evar DelegateIDs
+                (fun (idx : Fin.t DelegateIDs)=>
+                   Vector.t consSig (numDelegateConstructors idx))
+      ltac:(fun DelegateConstructorSigs' =>
+    Iterate_Dep_Type_BoundedIndex_evar DelegateIDs
+                (fun (idx : Fin.t DelegateIDs)=>
+                   Vector.t methSig (numDelegateMethods idx))
+      ltac:(fun DelegateMethodSigs' =>
+        let DelegateConstructorSigs :=
+            constr:(Lookup_Iterate_Dep_Type
+                      (fun (idx : Fin.t DelegateIDs)=>
+                         Vector.t consSig (numDelegateConstructors idx))
+                      DelegateConstructorSigs') in
+        let DelegateMethodSigs :=
+            constr:(Lookup_Iterate_Dep_Type
+                      (fun (idx : Fin.t DelegateIDs)=>
+                         Vector.t methSig (numDelegateMethods idx))
+                      DelegateMethodSigs') in
+        let DelegateSigs :=
+            constr:(fun idx =>
+                      BuildADTSig (DelegateConstructorSigs idx) (DelegateMethodSigs idx)) in
+    Iterate_Dep_Type_BoundedIndex_evar DelegateIDs
+                          (fun (idx : Fin.t DelegateIDs) =>
+                             ilist (B := consDef (Rep := AbstractReps idx))
+                                   (DelegateConstructorSigs idx))
+      ltac:(fun DelegateConstructorSpecs' =>
+    Iterate_Dep_Type_BoundedIndex_evar DelegateIDs
+                (fun (idx : Fin.t DelegateIDs) =>
+                  ilist (B := methDef (Rep := AbstractReps idx))
+                        (DelegateMethodSigs idx))
+      ltac:(fun DelegateMethodSpecs' =>
+        let DelegateConstructorSpecs :=
+            constr:(Lookup_Iterate_Dep_Type
+                      (fun (idx : Fin.t DelegateIDs) =>
+                         ilist (B := consDef (Rep := AbstractReps idx))
+                               (DelegateConstructorSigs idx))
+                      DelegateConstructorSpecs') in
+        let DelegateMethodSpecs :=
+            constr:(Lookup_Iterate_Dep_Type
+                      (fun (idx : Fin.t DelegateIDs) =>
+                         ilist (B := methDef (Rep := AbstractReps idx))
+                               (DelegateMethodSigs idx))
+                      DelegateMethodSpecs') in
+        let DelegateSpecs :=
+            constr:(fun idx =>
+                      BuildADT
+                        (DelegateConstructorSpecs idx)
+                        (DelegateMethodSpecs idx)) in
+        ilist_of_evar'
+          n
+          (forall idx : Fin.t DelegateIDs,
+              ADT (DelegateSigs idx))
+          (fun (DelegateImpls : forall idx, ADT (DelegateSigs idx))
+                    (Sig : consSig) =>
+                  constructorType
+                    (dRepT (fun idx => Rep (DelegateImpls idx)))
+                    (consDom Sig))
+        consSigs
+        ltac:(fun cCons =>
+        ilist_of_evar'
+          n'
+          (forall idx : Fin.t DelegateIDs,
+              ADT (DelegateSigs idx))
+          (fun (DelegateImpls : forall idx, ADT (DelegateSigs idx))
+                    (Sig : methSig) =>
+                  methodType
+                    (dRepT (fun idx => Rep (DelegateImpls idx)))
+                    (methDom Sig)
+                    (methCod Sig)
+          )
+        methSigs
+        ltac:(fun cMeths =>
+        eapply (@Sharpen_w_Delegates
+                          DelegateIDs AbstractReps dRepT n n'
+                          consSigs methSigs
+                          consDefs methDefs
+                          numDelegateConstructors
+                          DelegateConstructorSigs
+                          numDelegateMethods
+                          DelegateMethodSigs
+                          DelegateConstructorSpecs
+                          DelegateMethodSpecs
+                          dAbsR
+                          cCons
+                          cMeths
+
+           )))))))))
+  end; try (simpl; repeat split; intros; subst).
+
+(* Determines if a term [r_o] is an abstract piece of state. *)
+Ltac identify_Abstract_Rep_Use r_o AbstractReps k :=
+  first [unify r_o (AbstractReps Fin.F1);
+          match type of AbstractReps with
+          | Fin.t ?n -> _ => k (@Fin.F1 (n - 1))
+          end
+        | identify_Abstract_Rep_Use r_o (fun n => AbstractReps (Fin.FS n))
+                                    ltac:(fun n => k (Fin.FS n))].
+
+(* Crawls through the goal to identify any occurences of abstract *)
+(* state. (Uber generic, albeit super inefficient. *)
+Ltac find_Abstract_Rep AbstractReps k :=
+  match goal with
+    |- context [?r_o] =>
+    identify_Abstract_Rep_Use
+      ltac:(type of r_o)
+             AbstractReps ltac:(k r_o)
+
+  end.
+
+Definition
+  Implement_Abstract_Operation
+  (* The 'abstract' ADT's representation type. *)
+  (AbstractRep : Type)
+
+  (* The signatures of each delegate's constructors *)
+  (* and methods in terms of the abstract representation *)
+  (* types. *)
+  (numDelegateConstructors : nat)
+  (DelegateConstructorSigs
+   : Vector.t consSig numDelegateConstructors)
+  (numDelegateMethods : nat)
+  (DelegateMethodSigs
+   : Vector.t methSig numDelegateMethods)
+  (DelegateSigs := BuildADTSig
+                     DelegateConstructorSigs
+                     DelegateMethodSigs)
+
+  (* The specifications of each delegate's constructors *)
+  (* and methods in terms of the abstract representation *)
+  (* types. *)
+  (DelegateConstructorSpecs
+   : ilist (B := @consDef AbstractRep) DelegateConstructorSigs)
+  (DelegateMethodSpecs
+   : ilist (B := methDef (Rep := AbstractRep)) DelegateMethodSigs)
+  (DelegateSpecs := BuildADT
+                      DelegateConstructorSpecs
+                      DelegateMethodSpecs)
+
+  (* The concrete ADT implementation's type. *)
+  (ConcreteRep : Type)
+  (DelegateImpl : ADT DelegateSigs)
+  (ValidImpl
+   : refineADT DelegateSpecs
+               DelegateImpl)
+  : forall midx
+           (c : methodType
+                  (AbstractRep)
+                  (fst (MethodDomCod DelegateSigs midx))
+                  (snd (MethodDomCod DelegateSigs midx))),
+    c = (Methods DelegateSpecs midx)
+    -> refineMethod (AbsR ValidImpl)
+                    c
+                    (Methods DelegateImpl midx).
+Proof.
+  intros; subst.
+  apply (ADTRefinementPreservesMethods ValidImpl midx).
+Qed.
+
+Fixpoint observerType' (rep : Type) (dom : list Type) (cod : option Type)
+         {struct dom} : Type :=
+  match dom with
+  | [] =>
+    match cod with
+    | Some cod' => Comp cod'
+    | None => Comp unit
+    end
+  | d :: dom' => d -> observerType' rep dom' cod
+  end.
+
+Definition observerType (rep : Type)
+           (dom : list Type)
+           (cod : option Type) :=
+  rep -> observerType' rep dom cod.
+
+Fixpoint refineObserver' {oldRep newRep}
+         (AbsR : oldRep -> newRep -> Prop)
+         (dom : list Type)
+         (cod : option Type) {struct dom} :=
+  match
+    dom as dom'
+    return
+    (observerType' oldRep dom' cod
+     -> methodType' newRep dom' cod
+     -> Prop)
+  with
+  | [] =>
+    match cod as cod' return
+          (observerType' oldRep [] cod' -> methodType' newRep [] cod' -> Prop)
+    with
+    | Some cod' =>
+      fun oldObserver newMethod =>
+        refine oldObserver
+               (r <- newMethod; ret (snd r))
+    | None =>
+      fun oldObserver newMethod =>
+        refine oldObserver (r <- newMethod; ret tt)
+    end
+  | D :: dom' =>
+    fun oldObserver newMethod =>
+      forall d : D, refineObserver' AbsR dom' cod (oldObserver d) (newMethod d)
+  end.
+
+Definition refineObserver {oldRep newRep}
+           (AbsR : oldRep -> newRep -> Prop)
+           (dom : list Type) (cod : option Type)
+           (oldObserver : observerType oldRep dom cod)
+           (newMethod : methodType newRep dom cod) :=
+  forall (r_o : oldRep) (r_n : newRep),
+    AbsR r_o r_n
+    -> refineObserver' AbsR dom cod (oldObserver r_o) (newMethod r_n).
+
+Lemma refineObserverTrans {oldRep newRep}
+  : forall (AbsR : oldRep -> newRep -> Prop)
+           (dom : list Type) (cod : option Type)
+           (oldObserver : observerType oldRep dom cod)
+           (oldMethod : methodType oldRep dom cod)
+           (newMethod : methodType newRep dom cod),
+    refineObserver eq oldObserver oldMethod
+    -> refineMethod AbsR oldMethod newMethod
+    -> refineObserver AbsR oldObserver newMethod.
+Proof.
+  unfold refineObserver; induction dom; simpl.
+  - destruct cod; intros.
+    + rewrite H by eauto.
+      setoid_rewrite <- H0; eauto.
+      repeat setoid_rewrite refineEquiv_bind_bind; f_equiv.
+      intro.
+      setoid_rewrite refineEquiv_bind_unit; simpl.
+      intros v Comp_v; computes_to_inv; subst; computes_to_econstructor.
+    + rewrite H by eauto.
+      setoid_rewrite <- H0; eauto.
+      repeat setoid_rewrite refineEquiv_bind_bind; f_equiv.
+      intro.
+      intros v Comp_v; computes_to_inv; subst; computes_to_econstructor.
+  - intros.
+    eapply IHdom with
+    (oldObserver := fun r_o => oldObserver r_o d)
+      (oldMethod := fun r_o => oldMethod r_o d)
+      (newMethod := fun r_n => newMethod r_n d);
+      intros; subst; eauto.
+    unfold refineMethod; intros; eapply H0; eauto.
+Qed.
+
+Fixpoint liftObserverToMethod'
+         (rep : Type)
+         (dom : list Type)
+         (cod : option Type)
+         (observer : observerType' rep dom cod)
+         (r : rep)
+         {struct dom}
+  : methodType' rep dom cod :=
+  match dom as dom' return
+        observerType' rep dom' cod
+        -> methodType' rep dom' cod
+  with
+  | [] =>
+    match cod as cod' return
+          observerType' rep [ ] cod'
+          -> methodType' rep [ ] cod' with
+    | Some cod' => fun observer => r' <- observer; ret (r, r')
+    | None => fun observer => r' <- observer; ret r
+    end
+  | D :: dom' =>
+    fun observer' (d : D) =>
+      liftObserverToMethod' dom' cod (observer' d) r
+  end observer.
+
+Definition liftObserverToMethod
+           (rep : Type)
+           (dom : list Type)
+           (cod : option Type)
+           (observer : observerType rep dom cod) :=
+  fun r => liftObserverToMethod' dom cod (observer r) r.
+
+Lemma refineObserverLift {oldRep}
+  : forall (dom : list Type) (cod : option Type)
+           (oldObserver : observerType oldRep dom cod),
+    refineObserver eq oldObserver (liftObserverToMethod oldObserver).
+Proof.
+  unfold refineObserver, liftObserverToMethod; induction dom; simpl.
+  - destruct cod; intros.
+    + rewrite H by eauto.
+      intros v Comp_v; computes_to_inv; subst; simpl; eauto.
+    + rewrite H by eauto.
+      intros v Comp_v; computes_to_inv; subst; simpl; eauto.
+      destruct v1; eauto.
+  - intros.
+    eapply IHdom with
+    (oldObserver := fun r_o => oldObserver r_o d);
+      intros; subst; eauto.
+Qed.
+
+Definition
+  Implement_Abstract_Observer
+  (* The 'abstract' ADT's representation type. *)
+  (AbstractRep : Type)
+
+  (* The signatures of each delegate's constructors *)
+  (* and methods in terms of the abstract representation *)
+  (* types. *)
+  (numDelegateConstructors : nat)
+  (DelegateConstructorSigs
+   : Vector.t consSig numDelegateConstructors)
+  (numDelegateMethods : nat)
+  (DelegateMethodSigs
+   : Vector.t methSig numDelegateMethods)
+  (DelegateSigs := BuildADTSig
+                     DelegateConstructorSigs
+                     DelegateMethodSigs)
+
+  (* The specifications of each delegate's constructors *)
+  (* and methods in terms of the abstract representation *)
+  (* types. *)
+  (DelegateConstructorSpecs
+   : ilist (B := @consDef AbstractRep) DelegateConstructorSigs)
+  (DelegateMethodSpecs
+   : ilist (B := methDef (Rep := AbstractRep)) DelegateMethodSigs)
+  (DelegateSpecs := BuildADT
+                      DelegateConstructorSpecs
+                      DelegateMethodSpecs)
+
+  (* The delegate ADT implementation. *)
+  (DelegateImpl : ADT DelegateSigs)
+  (ValidImpl
+   : refineADT DelegateSpecs DelegateImpl)
+  : forall midx
+           (c : observerType
+                  (AbstractRep)
+                  (fst (MethodDomCod DelegateSigs midx))
+                  (snd (MethodDomCod DelegateSigs midx))),
+    refineObserver eq c (Methods DelegateSpecs midx)
+    -> refineObserver (AbsR ValidImpl)
+                      c
+                      (Methods DelegateImpl midx).
+Proof.
+  intros; subst.
+  eapply refineObserverTrans; eauto.
+  eapply (ADTRefinementPreservesMethods ValidImpl midx).
+Qed.
+
+Opaque UpdateUnConstrRelationInsertC.
+Opaque UpdateUnConstrRelationDeleteC.
+
+Ltac doOne srewrite_fn drills_fn finish_fn :=
+  first [srewrite_fn | drills_fn | finish_fn].
+
+Definition SharpenedScheduler :
+  {adt' : _ & refinedUnderDelegates SchedulerSpec adt'}.
+Proof.
+  eexists; unfold SchedulerSpec.
   simpl; pose_string_hyps; pose_heading_hyps.
-  start_honing_QueryStructure'.
-  hone method "Spawn".
-  { setoid_rewrite UniqueAttribute_symmetry.
-    setoid_rewrite (@refine_uniqueness_check_into_query' SchedulerSchema Fin.F1 _ _ _ _).
-    setoid_rewrite refine_For_rev.
-    setoid_rewrite refine_Count.
-    simplify with monad laws; simpl in *; subst.
-    setoid_rewrite refine_pick_eq'.
-    setoid_rewrite refine_bind_unit.
-    setoid_rewrite refine_If_Then_Else_Duplicate.
-    finish honing. }
+  eapply refinedUnderDelegatesStep.
+  eapply SharpenStep;
+    [ match goal with
+        |- context [@BuildADT (QueryStructure ?Rep) _ _ _ _ _ _] =>
+        eapply refineADT_BuildADT_Rep_refine_All with (AbsR := @DropQSConstraints_AbsR Rep);
+          [ repeat (first [eapply refine_Constructors_nil
+                          | eapply refine_Constructors_cons;
+                            [ simpl; intros;
+                              match goal with
+                              | |- refine _ (?E _ _ _ _) => let H := fresh in set (H := E)
+                              | |- refine _ (?E _ _ _) => let H := fresh in set (H := E)
+                              | |- refine _ (?E _ _) => let H := fresh in set (H := E)
+                              | |- refine _ (?E _) => let H := fresh in set (H := E)
+                              | |- refine _ (?E) => let H := fresh in set (H := E)
+                              | _ => idtac
+                              end;
+                              (* Drop constraints from empty *)
+                              try apply Constructor_DropQSConstraints;
+                              cbv delta [GetAttribute] beta; simpl
+                            | ] ])
+          | repeat (first [eapply refine_Methods_nil
+                          | eapply refine_Methods_cons;
+                            [ simpl; intros;
+                              match goal with
+                              | |- refine _ (?E _ _ _ _) => let H := fresh in set (H := E)
+                              | |- refine _ (?E _ _ _) => let H := fresh in set (H := E)
+                              | |- refine _ (?E _ _) => let H := fresh in set (H := E)
+                              | |- refine _ (?E _) => let H := fresh in set (H := E)
+                              | |- refine _ (?E) => let H := fresh in set (H := E)
+                              | _ => idtac
+                              end;
+                              cbv delta [GetAttribute] beta; simpl | ]
+          ])]
+      end | ].
+  - doAny drop_constraints
+          master_rewrite_drill ltac:(repeat subst_refine_evar; try finish honing).
+  - doAny drop_constraints
+          master_rewrite_drill ltac:(repeat subst_refine_evar; try finish honing).
+  - doAny drop_constraints
+          master_rewrite_drill ltac:(repeat subst_refine_evar; try finish honing).
+  - hone method StringId0.
+    { setoid_rewrite UniqueAttribute_symmetry.
+      setoid_rewrite (@refine_uniqueness_check_into_query' SchedulerSchema Fin.F1 _ _ _ _).
+      simpl.
+      setoid_rewrite refine_For_rev.
+      setoid_rewrite refine_Count.
+      subst.
+      simplify with monad laws.
+      repeat doOne ltac:(first [
+                             rewrite !refine_if_If
+                           | rewrite refine_If_Then_Else_Duplicate])
+                          master_rewrite_drill ltac:(repeat subst_refine_evar; try finish honing).
+    }
+    hone representation using (@FiniteTables_AbsR SchedulerSchema).
+    + simplify with monad laws.
+      refine pick val _; simpl; intuition.
+      eauto using FiniteTables_AbsR_QSEmptySpec.
+    + repeat doOne simplify_queries
+             Finite_AbsR_rewrite_drill ltac:(repeat subst_refine_evar; try finish honing).
+    + repeat doOne simplify_queries
+             Finite_AbsR_rewrite_drill ltac:(repeat subst_refine_evar; try finish honing).
+    + repeat doOne simplify_queries
+             Finite_AbsR_rewrite_drill ltac:(repeat subst_refine_evar; try finish honing).
+    + hone representation using (@UnConstryQueryStructure_Abstract_AbsR SchedulerSchema).
+      * simplify with monad laws.
+        refine pick val (imap2 rawRel (Build_EmptyRelations (qschemaSchemas SchedulerSchema))).
+        finish honing.
+        unfold UnConstryQueryStructure_Abstract_AbsR; simpl; intuition.
+      * Transparent UpdateUnConstrRelationInsertC.
+        Transparent UpdateUnConstrRelationDeleteC.
+        doAny parameterize_query_structure
+              rewrite_drill ltac:(repeat subst_refine_evar; try finish honing).
+      * doAny parameterize_query_structure
+              rewrite_drill ltac:(repeat subst_refine_evar; try finish honing).
+      * doAny parameterize_query_structure
+              rewrite_drill ltac:(repeat subst_refine_evar; try finish honing).
+      * eapply reflexivityT.
+  - simpl.
+    FullySharpenEachMethod_w_Delegates
+      1
+      (fun idx : Fin.t (numRawQSschemaSchemas SchedulerSchema) =>
+         @IndexedEnsemble (@RawTuple (rawSchemaHeading (Vector.nth (qschemaSchemas SchedulerSchema) idx))))
+      (@Iterate_Dep_Type_BoundedIndex 1)
+      (@Iterate_Dep_Type_AbsR 1).
+    Focus 2.
+
+simplify with monad laws; simpl.
+etransitivity.
+apply refine_under_bind_both.
+
+Ltac find_AbsR DelegateImpls ValidImpls :=
+find_Abstract_Rep
+  (fun idx : Fin.t (numRawQSschemaSchemas SchedulerSchema) =>
+     @IndexedEnsemble (@RawTuple (rawSchemaHeading (Vector.nth (qschemaSchemas SchedulerSchema) idx))))
+  ltac:(fun r_o n =>
+          (* Synthesize a similar concrete representation type [r_n'] *)
+          (* using an evar. If this fails, we don't have a candidate for*)
+          (* operation conversion. *)
+          makeEvar (Rep (DelegateImpls n))
+                              ltac:(fun r_n' =>
+                                      let AbsR_r_o := fresh in
+                                      assert (AbsR (ValidImpls n) r_o r_n')
+                                        as AbsR_r_o by intuition eauto);
+        (* Generalize the refineADT proof for the concrete representation*)
+        (* type [r_n'] so that we can add a new method to its spec. *)
+        let ValidImplT' := (type of (ValidImpls n)) in
+        let ValidImplT := (eval simpl in ValidImplT') in
+        pose (ValidImpls n : ValidImplT)
+       ).
+
+find_AbsR DelegateImpls ValidImpls.
+
+
+    match goal with
+      H : refineADT (@BuildADT ?Rep ?n ?n' ?consSigs ?methSigs ?consDefs ?methDefs)
+                _
+  |- refine ?c ?H0 =>
+  makeEvar nat
+    ltac:(fun n'' =>
+  makeEvar (Vector.t methSig n'')
+     ltac:(fun methSigs' =>
+  makeEvar (ilist (B := @methDef Rep) methSigs')
+           ltac:(fun methDefs' =>
+                   unify methSigs
+                         (@Vector.cons methSig {| methID := "foo";
+                              methDom := @nil Type;
+                              methCod := Some (nat : Type) |} n'' methSigs');
+             unify methDefs
+                   (@icons methSig
+                           (@methDef Rep)
+                           {| methID := "foo";
+                              methDom := @nil Type;
+                              methCod := Some (nat : Type) |}
+                           n'' methSigs'
+                           (@Build_methDef Rep {| methID := "foo";
+                              methDom := @nil Type;
+                              methCod := Some (nat : Type) |}
+                                           (fun (r_o : Rep) =>
+                                              idx <- { idx | UnConstrFreshIdx r_o idx};
+                                            ret (r_o, idx)))
+                           methDefs');
+             apply (@Implement_Abstract_Observer Rep
+                                                  n consSigs (S n'')
+                                                 methSigs
+                                                 consDefs
+                                                 methDefs
+                                                 _
+                                                 (ValidImpls (Fin.F1))
+                                                 (Fin.F1)
+                                                 _
+                                                 (refineObserverLift _)
+                                                 
+                  )
+         ); eauto))
+end.
+intros.
+rewrite !refine_For.
+Transparent QueryResultComp.
+
+simplify with monad laws.
+apply refine_under_bind_both.
+find_AbsR DelegateImpls ValidImpls.
+
+apply r0.
+simpl in r0.
+Check (r0 _ (refineObserverLift _)).
+unfold refineObserver in r0; simpl in r0.
+
+
+
   (* Now we implement the various set operations using BagADTs. *)
   - make_simple_indexes
       {|
-      prim_fst := [ ("EqualityIndex", Fin.F1);
-                    ( "EqualityIndex", Fin.FS (@Fin.F1 1) ) ];
-      prim_snd := () |}
-               ltac:(LastCombineCase6 BuildEarlyEqualityIndex)
-                      ltac:(LastCombineCase5 BuildLastEqualityIndex).
+        prim_fst := [ ("EqualityIndex", Fin.F1);
+                      ( "EqualityIndex", Fin.FS (@Fin.F1 1) ) ];
+        prim_snd := () |}
+      ltac:(LastCombineCase6 BuildEarlyEqualityIndex)
+             ltac:(LastCombineCase5 BuildLastEqualityIndex).
     + plan EqIndexUse createEarlyEqualityTerm createLastEqualityTerm
            EqIndexUse_dep createEarlyEqualityTerm_dep createLastEqualityTerm_dep.
     + plan EqIndexUse createEarlyEqualityTerm createLastEqualityTerm
